Iris/Iris/Algebra/Heap.lean
@@ -6,7 +6,6 @@ Authors: Markus de Medeiros, Puming Liu
 module
 
 public import Iris.Algebra.CMRA
-public import Iris.Algebra.LocalUpdates
 public import Iris.Algebra.OFE
 public import Iris.Algebra.IsOp
 public import Iris.Algebra.LocalUpdates
